io/Compiler.Model1.fst
@@ -11,54 +11,6 @@ include Compiler.Languages
 include Compiler.MIO.To.Interm
 open MIO.Behavior
 
-let static_cmd
-  (#mst:mst)
-  caller
-  (cmd : io_cmds)
-  (arg : io_sig.args cmd) :
-  MIO (io_sig.res cmd arg) mst IOActions
-    (requires (fun h -> io_pre cmd arg h))
-    (ensures (fun h (r:io_sig.res cmd arg) lt ->
-        io_post cmd arg r /\
-        lt == [convert_call_to_event caller cmd arg r])) =
-  MIOwp?.reflect (MIO.Sig.Call.mio_call caller cmd arg)
-
-type io_lib (fl:erased tflag) (pi:policy_spec) (mst:mst) (c:caller) =
-  (cmd : io_cmds) ->
-  (arg : io_sig.args cmd) ->
-  MIO (io_resm cmd arg) mst fl
-    (requires (fun _ -> True))
-    (ensures (fun h r lt ->
-      enforced_locally pi h lt /\
-      (match r with
-       | Inr Contract_failure -> lt == []
-       | r' -> io_post cmd arg r' /\ lt == [convert_call_to_event c cmd arg r'])))
-
-type io_lib' (fl:erased tflag) (#pi:policy_spec) (mst:mst) (phi:policy mst pi) (c:caller) =
-  (cmd : io_cmds) ->
-  (arg : io_sig.args cmd) ->
-  MIO (io_resm cmd arg) mst fl
-    (requires (fun _ -> True))
-    (ensures (fun h r lt ->
-      enforced_locally pi h lt /\
-      //enforced_locally (fun h _ cmd arg -> phi h cmd arg) h lt /\
-      // ^ really needed?
-      (match r with
-       | Inr Contract_failure -> lt == []
-       | r' -> io_post cmd arg r' /\ lt == [convert_call_to_event c cmd arg r'])))
-
-#push-options "--compat_pre_core 1" // fixme
-val inst_io_cmds : #mst:mst -> #pi:policy_spec -> phi:policy mst pi -> io_lib' AllActions mst phi Ctx
-let inst_io_cmds phi cmd arg =
-  let s0 = get_state () in
-  if phi s0 cmd arg then (
-    // Need the letbinding here it won't typecheck... why?
-    let r : io_resm' cmd arg = static_cmd Ctx cmd arg in
-    // assume (io_post cmd arg r) ; // Even that's not enough
-    r
-  ) else Inr Contract_failure
-#pop-options
-
 (** **** interfaces **)
 noeq
 type src_interface = {
